Lift [Int.positive_part].

lib/zoo_std/int.ml
@@ -1,3 +1,6 @@
+type t =
+  int
+
 let min =
   Stdlib.Int.min
 [@@zoo.overwrite
@@ -11,3 +14,6 @@ let max =
   fun n1 n2 ->
     if n1 < n2 then n2 else n1
 ]
+
+let positive_part t =
+  max 0 t
