lib/zoo_std/int.mli
@@ -1,4 +1,10 @@
+type t =
+  int
+
 val min :
   int -> int -> int
 val max :
   int -> int -> int
+
+val positive_part :
+  int -> int
